Final Cleanup for 12/4 push

affine/old/affine_coordinate_framed_space.lean
@@ -3,15 +3,6 @@ import linear_algebra.basis
 import .affine_coordinate_space
 import data.real.basic
 
-/-
-This file contains
-affine_tuple_coord_frame
-affine_coord_frame
-aff_coord_pt
-aff_coord_vec
-Also all instances necessary. Missing some proofs 11/20
--/
-
 
 
 open list
@@ -45,80 +36,35 @@ variables
 An affine frame comprises an origin point
 and a basis for the vector space.
 -/
-structure affine_tuple_coord_frame
-(K : Type w)
-(n : ℕ)
-[inhabited K]
-[field K]  :=
-mk ::
-    (origin : aff_pt_coord_tuple K n) 
-    (basis : (fin n) → aff_vec_coord_tuple K n) 
-    (proof_is_basis : is_basis K basis) 
+structure affine_frame  :=
+(origin : X) 
+(basis : ι → V) 
+(proof_is_basis : is_basis K basis)
 
-inductive affine_coord_frame
-(K : Type w)
-(n : ℕ)
-[inhabited K]
-[field K]
-| tuple (base : affine_tuple_coord_frame K n) 
-: affine_coord_frame
-| derived 
-    (origin : aff_pt_coord_tuple K n) 
-    (basis : (fin n) → aff_vec_coord_tuple K n) 
-    (proof_is_basis : is_basis K basis) 
-(base : affine_coord_frame)
-: affine_coord_frame
+#check affine_frame
 /-
-structure affine_derived_coord_frame extends 
-    affine_tuple_coord_frame K n :=
-mk ::
-    (base : affine_tuple_coord_frame K n)
--/
-instance: has_lift (affine_derived_coord_frame K n) (affine_tuple_coord_frame K n) := ⟨sorry⟩
-
-/-
-inductive affine_coord_frame 
-(K : Type w)
-(n : ℕ)
-[inhabited K]
-[field K] : affine_tuple_coord_frame K n → Type
-| standard 
-: affine_coord_frame
---(origin : X) 
---(basis : (fin n) → aff_vec_coord_tuple K n) 
---(proof_is_basis : is_basis K basis) : affine_coord_frame
-| derived 
-    (origin : aff_pt_coord_tuple K n) 
-    (basis : (fin n) → aff_vec_coord_tuple K n) 
-    (proof_is_basis : is_basis K basis) 
-    (fr : affine_coord_frame)
-    : affine_coord_frame
--/
-/-
-mutual inductive affine_coord_frame, aff_coord_pt, aff_coord_vec
-with affine_coord_frame : Type
+mutual inductive affine_coordinate_frame, aff_coord_pt, aff_coord_vec
+with affine_coordinate_frame : Type
 | std_frame 
 | gen_frame 
     (origin : aff_coord_pt) 
     (basis : ι → aff_coord_vec) 
     (proof_is_basis : is_basis K basis)
-with aff_coord_pt : affine_coord_frame X K V ι →  Type
+with aff_coord_pt : affine_coordinate_frame X K V ι →  Type
 | mk (tuple : aff_pt_coord_tuple K n)
-with aff_coord_vec : affine_coord_frame X K V ι → Type
+with aff_coord_vec : affine_coordinate_frame X K V ι → Type
 | mk (tuple : aff_vec_coord_tuple K n)
 -/
 
-structure aff_coord_pt (fr : affine_coord_frame K n) 
-            extends aff_pt_coord_tuple K n :=
+structure aff_coord_pt (fr : affine_frame X K V ι) extends aff_pt_coord_tuple K n :=
    -- (tuple : aff_pt_coord_tuple K n)
    mk ::
 
-structure aff_coord_vec (fr : affine_coord_frame K n) 
-            extends aff_vec_coord_tuple K n  :=
+structure aff_coord_vec (fr : affine_frame X K V ι) extends aff_vec_coord_tuple K n  :=
    -- (tuple : aff_vec_coord_tuple K n)
    mk ::
 /-
-def affine_coord_frame_origin (frame : affine_coord_frame X K V ι) :=
+def affine_coordinate_frame_origin (frame : affine_coordinate_frame X K V ι) :=
 match frame with
 | std_frame := _
 | gen_frame o b pf := o
@@ -131,9 +77,9 @@ def frame_basis : affine_frame X K V ι → (ι → V) :=
 
 
 variables 
-    (fr : affine_coord_frame K n) 
-    (cv1 cv2 : aff_coord_vec K n fr) 
-    (cp1 cp2 : aff_coord_pt  K n fr)
+    (fr : affine_frame X K V ι) 
+    (cv1 cv2 : aff_coord_vec X K V n ι fr) 
+    (cp1 cp2 : aff_coord_pt  X K V n ι fr)
 
 /-
 -- lemmas so that the following operations are well-defined
@@ -220,26 +166,26 @@ simp only [x_fst_zero, neg_zero, head_0],
 end
 
 -/
-def vec_add_coord : aff_coord_vec K n fr → aff_coord_vec K n fr → aff_coord_vec K n fr :=
+def vec_add_coord : aff_coord_vec X K V n ι fr → aff_coord_vec X K V n ι fr → aff_coord_vec X K V n ι fr :=
     λ x y, ⟨⟨ladd x.1.l y.1.l, list_sum_fixed K n x.1 y.1, sum_fst_fixed K n x.1 y.1⟩⟩
-def vec_zero_coord : aff_coord_vec K n fr := ⟨⟨zero_vector K n, len_zero K n, head_zero K n⟩⟩
-def vec_neg_coord : aff_coord_vec K n fr → aff_coord_vec K n fr
+def vec_zero_coord : aff_coord_vec X K V n ι fr := ⟨⟨zero_vector K n, len_zero K n, head_zero K n⟩⟩
+def vec_neg_coord : aff_coord_vec X K V n ι fr → aff_coord_vec X K V n ι fr
 | ⟨⟨l, len, fst⟩⟩ := ⟨⟨vecl_neg l, vec_len_neg K n ⟨l, len, fst⟩, head_neg_0 K n ⟨l, len, fst⟩⟩⟩
 
 
 /-! ### type class instances for the abelian group operations -/
-instance : has_add (aff_coord_vec K n fr) := ⟨vec_add_coord K n fr⟩
-instance : has_zero (aff_coord_vec K n fr) := ⟨vec_zero_coord K n fr⟩
-instance : has_neg (aff_coord_vec K n fr) := ⟨vec_neg_coord K n fr⟩
+instance : has_add (aff_coord_vec X K V n ι fr) := ⟨vec_add_coord X K V n ι fr⟩
+instance : has_zero (aff_coord_vec X K V n ι fr) := ⟨vec_zero_coord X K V n ι fr⟩
+instance : has_neg (aff_coord_vec X K V n ι fr) := ⟨vec_neg_coord X K V n ι fr⟩
 @[ext]
-def vec_scalar_coord : K → aff_coord_vec K n fr → aff_coord_vec K n fr :=
+def vec_scalar_coord : K → aff_coord_vec X K V n ι fr → aff_coord_vec X K V n ι fr :=
     λ a x, ⟨⟨scalar_mul a x.1.1, trans (scale_len a x.1.1) x.1.2, sorry⟩⟩
 /-! ### Type class instance for abelian group -/
-instance aff_comm_group_coord : add_comm_group (aff_coord_vec K n fr) :=
+instance aff_comm_group_coord : add_comm_group (aff_coord_vec X K V n ι fr) :=
 begin
     sorry
 end
-instance : has_scalar K (aff_coord_vec K n fr) := ⟨vec_scalar_coord K n fr⟩
+instance : has_scalar K (aff_coord_vec X K V n ι fr) := ⟨vec_scalar_coord X K V n ι fr⟩
 
 /-
 lemma vec_one_smul_coord : (1 : K) • cv1 = cv1 := 
@@ -259,35 +205,35 @@ rw one_smul_cons,
 exact a_1,
 end
 -/
-lemma vec_mul_smul_coord : ∀ g h : K, ∀ x : aff_coord_vec K n fr, (g * h) • x = g • h • x := sorry
+lemma vec_mul_smul_coord : ∀ g h : K, ∀ x : aff_coord_vec X K V n ι fr, (g * h) • x = g • h • x := sorry
 
 
-instance : mul_action K (aff_coord_vec K n fr) := ⟨sorry, vec_mul_smul_coord K n fr⟩
+instance : mul_action K (aff_coord_vec X K V n ι fr) := ⟨sorry, vec_mul_smul_coord X K V n ι fr⟩
 
 
-instance : distrib_mul_action K (aff_coord_vec K n fr) := 
+instance : distrib_mul_action K (aff_coord_vec X K V n ι fr) := 
     sorry
-instance aff_semimod_coord : semimodule K (aff_coord_vec K n fr)
-    --[distrib_mul_action K (aff_coord_vec K n fr)] 
+instance aff_semimod_coord : semimodule K (aff_coord_vec X K V n ι fr)
+    --[distrib_mul_action K (aff_coord_vec X K V n ι fr)] 
     := 
     -- extremely odd that this doesnt work....
     ⟨sorry, sorry⟩
 
 
 
-def aff_group_action_coord : (aff_coord_vec K n fr) → (aff_coord_pt K n fr) → (aff_coord_pt K n fr) :=
+def aff_group_action_coord : (aff_coord_vec X K V n ι fr) → (aff_coord_pt X K V n ι fr) → (aff_coord_pt X K V n ι fr) :=
     λ x y, ⟨⟨ladd x.1.1 y.1.1, sorry, sorry⟩⟩
 
-def aff_group_sub_coord : (aff_coord_pt K n fr) → (aff_coord_pt K n fr) → (aff_coord_vec K n fr) :=
+def aff_group_sub_coord : (aff_coord_pt X K V n ι fr) → (aff_coord_pt X K V n ι fr) → (aff_coord_vec X K V n ι fr) :=
     λ x y, ⟨⟨ladd x.1.1 (vecl_neg y.1.1), sorry, sorry⟩⟩
 
 
 
-instance : has_vadd (aff_coord_vec K n fr) (aff_coord_pt K n fr) := ⟨aff_group_action_coord K n fr⟩
+instance : has_vadd (aff_coord_vec X K V n ι fr) (aff_coord_pt X K V n ι fr) := ⟨aff_group_action_coord X K V n ι fr⟩
 
-instance : has_vsub (aff_coord_vec K n fr) (aff_coord_pt K n fr) := ⟨aff_group_sub_coord K n fr⟩
+instance : has_vsub (aff_coord_vec X K V n ι fr) (aff_coord_pt X K V n ι fr) := ⟨aff_group_sub_coord X K V n ι fr⟩
 
-instance : add_action (aff_coord_vec K n fr) (aff_coord_pt K n fr) := sorry--⟨aff_group_action K n, aff_zero_sadd K n, aff_add_sadd K n⟩
+instance : add_action (aff_coord_vec X K V n ι fr) (aff_coord_pt X K V n ι fr) := sorry--⟨aff_group_action K n, aff_zero_sadd K n, aff_add_sadd K n⟩
 
 /-
 We need proof that given a frame f, 
@@ -313,11 +259,11 @@ def pt_plus_vec
     [module K V] 
     [vector_space K V] 
     [affine_space V X]
-    {fr : affine_coord_frame K n} :
-    (aff_coord_pt K n fr) → 
-    (aff_coord_vec K n fr) → 
-    (aff_coord_pt K n fr) 
-| p v := aff_group_action_coord K n fr v p
+    {fr : affine_frame X K V ι} :
+    (aff_coord_pt X K V n ι fr) → 
+    (aff_coord_vec X K V n ι fr) → 
+    (aff_coord_pt X K V n ι fr) 
+| p v := aff_group_action_coord X K V n ι fr v p
 
 notation
  pt +ᵥ v := pt_plus_vec pt v
@@ -334,22 +280,22 @@ def pt_minus_vec
     [module K V] 
     [vector_space K V] 
     [affine_space V X]
-    {fr : affine_coord_frame K n} :
-    (aff_coord_pt K n fr) → 
-    (aff_coord_vec K n fr) → 
-    (aff_coord_pt K n fr) 
-| p v := aff_group_action_coord K n fr (vec_neg_coord K n fr v) p
+    {fr : affine_frame X K V ι} :
+    (aff_coord_pt X K V n ι fr) → 
+    (aff_coord_vec X K V n ι fr) → 
+    (aff_coord_pt X K V n ι fr) 
+| p v := aff_group_action_coord X K V n ι fr (vec_neg_coord X K V n ι fr v) p
 .
 notation
  pt -ᵥ v := pt_minus_vec pt v
 
 
-def prf : affine_space (aff_coord_vec K n fr) (aff_coord_pt  K n fr) := sorry
+def prf : affine_space (aff_coord_vec X K V n ι fr) (aff_coord_pt  X K V n ι fr) := sorry
 
 instance afc : affine_space 
-    (aff_coord_vec K n fr) 
-    (aff_coord_pt  K n fr) := 
-    prf K n fr
+    (aff_coord_vec X K V n ι fr) 
+    (aff_coord_pt  X K V n ι fr) := 
+    prf X K V n ι fr
 
 
 /-
@@ -361,10 +307,7 @@ KEEP?
 
 /-
 Code to manufacture a standard basis for a given affine space.
-
-Unused 11/20 - pushed into lib for now
 -/
-/-
 abbreviation zero := zero_vector K n
 
 def list.to_basis_vec : fin n → list K := λ x, (zero K n).update_nth (x.1 + 1) 1
@@ -379,11 +322,9 @@ def std_basis : fin n → aff_vec_coord_tuple K n :=
 lemma std_is_basis : is_basis K (std_basis K n) := sorry
 
 def aff_coord_space_std_frame : 
-    affine_coord_frame K n := 
-           ⟨(pt_zero K n) 
-           ,(std_basis K n) 
-           , (std_is_basis K n)⟩
--/
+    affine_frame (aff_pt_coord_tuple K n) K (aff_vec_coord_tuple K n) (fin n) := 
+        ⟨pt_zero K n, std_basis K n, std_is_basis K n⟩
+
 --affine_frame (aff_coord_pt fr_n) K (aff_coord_pt fr_n) (iota)
 
 
