affine/affine_coordinate_transform.lean
@@ -1,0 +1,180 @@
+import .affine_coordinate_framed_space_lib --linear_algebra.affine_space.basic
+import 
+    linear_algebra.affine_space.affine_equiv 
+    linear_algebra.nonsingular_inverse
+    linear_algebra.matrix
+--    linear_algebra.
+
+open aff_fr
+open aff_lib
+universes u 
+variables 
+    (K : Type u)
+    (n : ℕ )
+    [inhabited K]
+    [field K]
+    (fr1 : affine_coord_frame K n) 
+    (fr2 : affine_coord_frame K n) 
+    (cv1 cv2 : aff_coord_vec K n fr1) 
+    (cp1 cp2 : aff_coord_pt  K n fr2)
+
+/-
+
+def affine_coord_frame.build_path
+    {K : Type v}
+    {n : ℕ}
+    [inhabited K] 
+    [field K] 
+    :  affine_coord_frame K n → 
+        list (affine_tuple_coord_frame K n)
+| (affine_coord_frame.tuple b) := [b]
+| (affine_coord_frame.derived o b p f) := 
+    ⟨o,b,p⟩::(affine_coord_frame.build_path f)
+
+def affine_coord_space.find_transform_path
+    {K : Type v}
+    {n : ℕ}
+    [inhabited K] 
+    [field K] 
+    {fr1 : affine_coord_frame K n}
+    (from_sp : affine_coord_space K n fr1)
+    {fr2 : affine_coord_frame K n}
+    (to_sp : affine_coord_space K n fr2)
+    : transform_path
+    := ⟨affine_coord_frame.build_path fr1, 
+    affine_coord_frame.build_path fr2⟩
+
+-/
+attribute [reducible]
+abbreviation square_matrix
+    (K : Type u)
+    (n : ℕ)
+    [inhabited K] 
+    [field K] 
+    := matrix (fin n) (fin n ) K
+ 
+attribute [reducible]
+abbreviation col_matrix
+    (K : Type u)
+    (n : ℕ)
+    [inhabited K] 
+    [field K] 
+    := matrix (fin n) (fin 1) K
+   
+
+abbreviation 
+    affine_coord_frame_transform 
+    := 
+    (aff_coord_pt K n fr1) 
+    ≃ᵃ[K] 
+    (aff_coord_pt K n fr2)
+
+abbreviation
+    affine_coord_space_transform
+    (sp1 : affine_coord_space K n fr1)
+    (sp2 : affine_coord_space K n fr2)
+    := 
+    affine_coord_frame_transform K n fr1 fr2
+
+def affine_coord_vec.as_matrix
+    {K : Type u}
+    {n : ℕ}
+    [inhabited K] 
+    [field K] 
+    {fr : affine_coord_frame K n}
+    (v : aff_coord_vec K n fr)
+    : col_matrix K n
+    :=
+    λ i one, (@aff_lib.coord_helper K n v.1.1).nth i
+
+def affine_coord_pt.as_matrix
+    {K : Type u}
+    {n : ℕ}
+    [inhabited K] 
+    [field K] 
+    {fr : affine_coord_frame K n}
+    (v : aff_coord_pt K n fr)
+    : col_matrix K n
+    :=
+    λ i one, (@aff_lib.coord_helper K n v.1.1).nth i
+
+#check 
+(rfl :(matrix (fin n) (fin 1) K) = (col_matrix K n))
+   -- (matrix (fin n) (fin 1) K)=(matrix (fin n) (fin 1) K))
+/-
+instance 
+    {K : Type u}
+    {n : ℕ}
+    [inhabited K] 
+    [field K] 
+    {fr : affine_coord_frame K n}
+    : has_lift (aff_coord_pt K n fr)
+                (matrix (fin n) (fin 1) K)
+    := ⟨affine_coord_pt.as_matrix⟩ 
+instance 
+    {K : Type u}
+    {n : ℕ}
+    [inhabited K] 
+    [field K] 
+    {fr : affine_coord_frame K n}
+    : has_lift (aff_coord_vec K n fr)
+                (matrix (fin n) (fin 1) K)
+    := ⟨affine_coord_vec.as_matrix⟩ 
+-/
+/-
+invalid definition, a declaration named 'matrix.has_lift' has already been declaredL
+-/
+
+def m : matrix (fin n) (fin n) K
+    := λ i j, 1
+
+def affine_coord_frame.to_basis_matrix
+    {K : Type u}
+    {n : ℕ}
+    [inhabited K] 
+    [field K] 
+    (fr : affine_coord_frame K n)
+    : square_matrix K n
+    := 
+    λ i j,
+    (aff_lib.affine_tuple_vec.get_coords  
+    (
+        (aff_lib.affine_coord_frame.basis_coords 
+            fr) j))
+    .nth i
+
+--def fold_transforms
+
+def affine_coord_space.to_transform
+    {K : Type u}
+    {n : ℕ}
+    [inhabited K] 
+    [field K] 
+    {fr1 : affine_coord_frame K n}
+    (from_sp : affine_coord_space K n fr1)
+    {fr2 : affine_coord_frame K n}
+    (to_sp : affine_coord_space K n fr2)
+    : affine_coord_space_transform K n fr1 fr2 from_sp to_sp
+    :=
+
+/-
+def affine_coord_frame.to_equiv
+    {K : Type u}
+    {n : ℕ}
+    [inhabited K] 
+    [field K] 
+    (fr : affine_coord_frame K n)
+    :-/
+/-
+structure equiv (α : Sort*) (β : Sort*) :=
+(to_fun    : α → β)
+(inv_fun   : β → α)
+(left_inv  : left_inverse inv_fun to_fun)
+(right_inv : right_inverse inv_fun to_fun)
+
+structure affine_equiv (k P₁ P₂ : Type*) {V₁ V₂ : Type*} [ring k]
+  [add_comm_group V₁] [semimodule k V₁] [add_torsor V₁ P₁]
+  [add_comm_group V₂] [semimodule k V₂] [add_torsor V₂ P₂] extends P₁ ≃ P₂ :=
+(linear : V₁ ≃ₗ[k] V₂)
+(map_vadd' : ∀ (p : P₁) (v : V₁), to_equiv (v +ᵥ p) = linear v +ᵥ to_equiv p)
+-/
